Cslib/Logics/Propositional/Semantics/Classical.lean
@@ -1,0 +1,157 @@
+/-
+Copyright (c) 2026 Thomas Waring. All rights reserved.
+Released under Apache 2.0 license as described in the file LICENSE.
+Authors: Thomas Waring
+-/
+module
+
+public import Cslib.Logics.Propositional.Semantics.Heyting
+
+/-! # Two-valued semantics -/
+
+namespace Cslib.Logic.PL
+
+open Theory Derivation InferenceSystem Proposition Valuation Bool
+
+universe u
+
+variable {Atom : Type u} [DecidableEq Atom] {T : Theory Atom}
+
+namespace Proposition
+
+def flip [Bot Atom] (v : Valuation Atom Bool) (A : Proposition Atom) :=
+  match v⟦A⟧ with
+  | true => A
+  | false => ¬A
+
+omit [DecidableEq Atom] in
+lemma flip_def [Bot Atom] (v : Valuation Atom Bool) (A : Proposition Atom) :
+    A.flip v = match v⟦A⟧ with
+      | true => A
+      | false => ¬ A := rfl
+
+def atoms : Proposition Atom → List Atom
+  | atom x => [x]
+  | and A B | or A B | impl A B => A.atoms ++ B.atoms
+
+variable (x : Atom) (A B : Proposition Atom)
+
+def derivationFlip [Bot Atom] [IsIntuitionistic T] [IsClassical T] (Γ : Ctx Atom)
+    (A : Proposition Atom) (v : Valuation Atom Bool) (h : ∀ x ∈ A.atoms, (atom x).flip v ∈ Γ) :
+    T.Derivation Γ (A.flip v) :=
+  match A with
+  | atom x => ass (h x <| by simp [atoms])
+  | Proposition.and A B => by
+    rw [flip, interp_and]
+    match hA : v⟦A⟧ with
+    | true =>
+      match hB : v⟦B⟧ with
+      | true =>
+        apply conjI
+        · rw [show A = A.flip v by simp [Proposition.flip, hA]]
+          exact A.derivationFlip Γ v (by grind [atoms])
+        · rw [show B = B.flip v by simp [Proposition.flip, hB]]
+          exact B.derivationFlip Γ v (by grind [atoms])
+      | false =>
+        apply implI
+        refine implE (A := B) ?_ ?_
+        · rw [show (B → ⊥) = B.flip v by simp [Proposition.flip, hB]]
+          exact B.derivationFlip _ v (by grind [atoms])
+        · apply conjE₂ (A := A); exact ass <| Finset.mem_insert_self ..
+    | false =>
+      apply implI
+      refine implE (A := A) ?_ ?_
+      · rw [show (A → ⊥) = A.flip v by simp [Proposition.flip, hA]]
+        exact A.derivationFlip _ v (by grind [atoms])
+      · apply conjE₁ (B := B); exact ass <| Finset.mem_insert_self ..
+  | Proposition.or A B => by
+    rw [flip, interp_or]
+    match hA : v⟦A⟧ with
+    | true =>
+      apply disjI₁
+      rw [show A = A.flip v by simp [flip, hA]]
+      exact A.derivationFlip Γ v (by grind [atoms])
+    | false =>
+      match hB : v⟦B⟧ with
+      | true =>
+        apply disjI₂
+        rw [show B = B.flip v by simp [flip, hB]]
+        exact B.derivationFlip Γ v (by grind [atoms])
+      | false =>
+        apply implI; apply disjE (ass <| Finset.mem_insert_self ..)
+        · refine implE (A := A) ?_ (ass <| Finset.mem_insert_self ..)
+          rw [show (A → ⊥) = A.flip v by simp [Proposition.flip, hA]]
+          exact A.derivationFlip _ v (by grind [atoms])
+        · refine implE (A := B) ?_ (ass <| Finset.mem_insert_self ..)
+          rw [show (B → ⊥) = B.flip v by simp [Proposition.flip, hB]]
+          exact B.derivationFlip _ v (by grind [atoms])
+  | impl A B => by
+    rw [flip, interp_impl]
+    match hA : v⟦A⟧ with
+    | true =>
+      match hB : v⟦B⟧ with
+      | true =>
+        apply implI
+        rw [show B = B.flip v by simp [Proposition.flip, hB]]
+        exact B.derivationFlip _ v (by grind [atoms])
+      | false =>
+        apply implI; apply implE (A := B)
+        · rw [show (B → ⊥) = B.flip v by simp [Proposition.flip, hB]]
+          exact B.derivationFlip _ v (by grind [atoms])
+        · apply implE (A := A) (ass <| Finset.mem_insert_self ..)
+          rw [show A = A.flip v by simp [flip, hA]]
+          exact A.derivationFlip _ v (by grind [atoms])
+    | false =>
+      simp only [himp, Bool.not_false, Bool.le_true, sup_of_le_right]
+      apply implI; apply implE (A := ⊥) (T.efq B |>.weak_ctx <| by grind)
+      refine implE (A := A) ?_ (ass <| Finset.mem_insert_self ..)
+      rw [show (A → ⊥) = A.flip v by simp [Proposition.flip, hA]]
+      exact A.derivationFlip _ v (by grind [atoms])
+
+def byCases [Bot Atom] [IsClassical T] {A B : Proposition Atom} {Γ : Ctx Atom}
+    (D : T⇓(insert A Γ ⊢ B)) (D' : T⇓(insert (¬ A) Γ ⊢ B)) : T⇓(Γ ⊢ B) :=
+  (lem A |>.weak_ctx (Δ := Γ) <| Finset.empty_subset ..).disjE D D'
+
+def derivationTautAux [Bot Atom] [IsIntuitionistic T] [IsClassical T] (xs : List Atom)
+    (Γ : Ctx Atom) (A : Proposition Atom) (hA : ∀ u : Valuation Atom Bool, u⟦A⟧ = true)
+    (v : Valuation Atom Bool) (hΓ : ∀ x ∈ A.atoms, x ∈ xs ∨ (atom x).flip v ∈ Γ) :
+    T.Derivation Γ A := by
+  have hA' : ∀ u : Valuation Atom Bool, A.flip u = A := by simp [flip, hA]
+  match xs with
+  | [] => exact hA' v ▸ derivationFlip Γ A v (by simpa using hΓ)
+  | x :: xs =>
+    apply byCases (A := atom x) (B := A) (Γ := Γ)
+    · let v' : Valuation Atom Bool := fun y => if x = y then true else v y
+      apply A.derivationTautAux xs (insert (atom x) Γ) hA v'
+      intro y hy
+      by_cases hxy : x = y
+      case pos => rw [←hxy, show (atom x).flip v' = atom x by simp [v', flip]]; grind
+      case neg =>
+        rw [show (atom y).flip v' = (atom y).flip v by simp [flip, v', hxy]]
+        grind
+    · let v' : Valuation Atom Bool := fun y => if x = y then false else v y
+      apply A.derivationTautAux xs (insert (¬ atom x) Γ) hA v'
+      intro y hy
+      by_cases hxy : x = y
+      case pos => rw [←hxy, show (atom x).flip v' = (¬ atom x) by simp [v', flip]]; grind
+      case neg =>
+        rw [show (atom y).flip v' = (atom y).flip v by simp [flip, v', hxy]]
+        grind
+
+def derivationTaut [Bot Atom] [IsIntuitionistic T] [IsClassical T] (A : Proposition Atom)
+    (hA : ∀ u : Valuation Atom Bool, u⟦A⟧ = true) : T⇓A :=
+  A.derivationTautAux A.atoms ∅ hA (fun _ => true) (fun _ hx => Or.inl hx)
+
+end Proposition
+
+lemma Theory.lt_iff {T T' : Theory Atom} :
+    T < T' ↔ T ≤ T' ∧ ∃ A ∈ T', ¬ DerivableIn T A := by
+  simp [LE.le, LT.lt, WeakerThan]
+
+-- theorem Theory.inconsistent_of_gt_CPL [Bot Atom] [IsIntuitionistic T] [IsClassical T]
+--   (h : CPL < T) :
+--     T.Inconsistent := by
+--   obtain ⟨hle, ⟨A, h, h'⟩⟩ := Theory.lt_iff.mp h
+
+
+end Cslib.Logic.PL
